wip: Introduce the third iteration of the FreeSpec formalism
TODO

theories/Stdlib/env.mli
@@ -1,4 +1,0 @@
-open Coqbase
-
-val getenv : Bytestring.t -> Bytestring.t option [@@impure]
-val setenv : Bytestring.t -> Bytestring.t -> unit [@@impure]
