theories/Core/Contract.v
@@ -2,7 +2,7 @@
  * Copyright (C) 2018–2019 ANSSI
  *
  * Contributors:
- * 2018–2019 Thomas Letan <thomas.letan@ssi.gouv.fr>
+ * 2018–2020 Thomas Letan <thomas.letan@ssi.gouv.fr>
  *
  * This program is free software: you can redistribute it and/or modify
  * it under the terms of the GNU General Public License as published by
@@ -25,7 +25,8 @@
     semantics (according to a certain definition of “correct”). *)
 
 From Coq Require Import Setoid Morphisms.
-From FreeSpec.Core Require Export Interface Impure Semantics Component.
+From ExtLib Require Import StateMonad MonadState MonadTrans.
+From FreeSpec.Core Require Import Interface Impure Semantics Component.
 
 #[local]
 Open Scope signature_scope.
@@ -73,9 +74,15 @@ Arguments callee_obligation [i Ω] (c ω) [α] (_ _).
 Definition const_witness {i} :=
   fun (u : unit) (α : Type) (e : i α) (x : α) => u.
 
-Definition no_caller_obligation {i Ω} (ω : Ω) (α : Type) (e : i α) : Prop := True.
+Inductive no_caller_obligation {i Ω} (ω : Ω) (α : Type) (e : i α) : Prop :=
+| mk_no_caller_obligation : no_caller_obligation ω α e.
 
-Definition no_callee_obligation {i Ω} (ω : Ω) (α : Type) (e : i α) (x : α) : Prop := True.
+Hint Constructors no_caller_obligation : freespec.
+
+Inductive no_callee_obligation {i Ω} (ω : Ω) (α : Type) (e : i α) (x : α) : Prop :=
+| mk_no_callee_obligation : no_callee_obligation ω α e x.
+
+Hint Constructors no_callee_obligation : freespec.
 
 Definition no_contract (i : interface) : contract i unit :=
   {| witness_update := const_witness
@@ -83,7 +90,7 @@ Definition no_contract (i : interface) : contract i unit :=
    ; callee_obligation := no_callee_obligation
    |}.
 
-(** A similar — and as simple — contract is the one that forbids the use of a
+(** A similar —and as simple— contract is the one that forbids the use of a
     given interface. *)
 
 Definition do_no_use {i Ω} (ω : Ω) (α : Type) (e : i α) : Prop := False.
@@ -93,6 +100,8 @@ Definition forbid_specs (i : interface) : contract i unit :=
    ; caller_obligation := do_no_use
    ; callee_obligation := no_callee_obligation
    |}.
+
+(** * Composing Contracts *)
 
 (** As we compose interfaces and operational semantics, we can easily compose
     contracts together, by means of the [cplus] operator. Given [i] and [j]
@@ -165,7 +174,7 @@ Definition store_update (s : Type) :=
     defined our contract, but in the meantime, we define its callee obligation.
 
     The logic of these callee obligations is as follows: [Get] is expected to
-    produce a result strictly equal to the witness, and we do not have any
+    produce a result strictly eqv to the witness, and we do not have any
     obligations about the result of [Put] (which belongs to [unit] anyway, so
     there is not much to tell). *)
 
@@ -195,518 +204,3 @@ Definition store_specs (s : Type) : contract (STORE s) s :=
     contracts are defined independently from impure computations and
     interfaces, we can actually define several contracts to consider
     different set of hypotheses. *)
-
-(** * Reasoning with Contracts *)
-
-(** ** Impure Computation Trustworthiness *)
-
-(** An impure computation [p] is said respectful wrt. a contract [c] in
-    accordance to a witness [ω] when it only uses primitives of [i] which
-    satisfies [c] obligations. *)
-
-Inductive respectful_impure `{MayProvide ix i} {α Ω} (c : contract i Ω) (ω : Ω) : impure ix α -> Prop :=
-
-(** - Given a term [x], the computation [local x] is always respectful wrt. [c]
-      in accordance to [ω], since it does not use any primitives. *)
-
-| respectful_local (x : α)
-  : respectful_impure c ω (local x)
-
-(** - Given a primitive [e] and a continuation [f], if
-
-      - [e] satisfies [c] caller obligation
-      - [f] computations are respectful wrt. [c] in accordance to [ω'], where
-        [ω'] is the witness updated after [e] interpretation
-
-      then the impure computation [request_then e f] is respectful wrt. [c] in
-      accordance to [ω]. *)
-
-| respectful_request_some {β}
-    (e : ix β) (f : β -> impure ix α)
-    (req : gen_caller_obligation c ω e)
-    (next : forall (x : β),
-        gen_callee_obligation c ω e x
-        -> respectful_impure c (gen_witness_update c ω e x) (f x))
-  : respectful_impure c ω (request_then e f).
-
-#[program]
-Instance respectful_impure_Proper
-  : Proper (equal ==> Basics.impl) (@respectful_impure ix i H α Ω c ω).
-
-Next Obligation.
-  add_morphism_tactic.
-  unfold Basics.impl.
-  intros p q equ.
-  revert ω.
-  induction equ; intros ω.
-  + auto.
-  + intros trust.
-    inversion trust; ssubst.
-    constructor.
-    ++ exact req.
-    ++ intros x q.
-       apply H0.
-       now apply next.
-Qed.
-
-(** As is, the definition of [respectful_impure] would force FreeSpec users to
-    unfold any impure computations they may combine together with [bind].  For
-    instance, proving a computation of the form [bind p (λ _, p)] is respectful
-    would require to prove [p] is respectful twice, for two different
-    witnesses.  Moreover, it could be challenging to know, when interactively
-    writing the proof script, when “the first [p]” stops, and when “the second
-    [p]” starts.
-
-    We need a way to compose proofs about impure computations the same way we
-    compose impure computations with [bind].  We do that with the
-    [respectful_run] predicate, which describes the potential outcomes of a
-    computation in terms of results and witnesses. *)
-
-Inductive respectful_run `{MayProvide ix i} {α Ω} (c : contract i Ω)
-  : impure ix α -> Ω -> Ω -> α -> Prop :=
-
-(** Given a term [x], and an initial witness [ω], a respectful run of
-    [local x] produced a result [x] and a witness state [ω]. *)
-
-| run_local (x : α) (ω : Ω)
-  : respectful_run c (local x) ω ω x
-
-(** Given an initial witness [ω], a primitive [e] which satisfies [c]
-    caller obligations, and a continuation [f], a result [x] for [e] which
-    satisfies [c] callee obligations, if we can show that there is a respectful
-    run of [f x] which produces a term [y] and a witness [ω'], then there is a
-    respectful run of [request_then e f] which produces a result [y] and a
-    witness [ω']. *)
-
-| run_request {β} (ω : Ω)
-    (e : ix β) (o_caller : gen_caller_obligation c ω e) (f : β -> impure ix α)
-    (x : β) (o_callee : gen_callee_obligation c ω e x)
-    (ω' : Ω) (y : α) (rec : respectful_run c (f x) (gen_witness_update c ω e x) ω' y)
-  : respectful_run c (request_then e f) ω ω' y.
-
-(** Given a contract [c] and a witness [ω] an impure computation [p] and a
-    continuation [f] if
-
-    - [p] is a respectful impure computation wrt. [c] in accordance to [ω], and
-    - for all result [x] and witness [ω'] produces by [p], [f x] is respectful,
-
-    then [bind p f] is respectful. *)
-
-Lemma respectful_bind_respectful_run `{MayProvide ix i} {α β Ω}
-  (c : contract i Ω) (ω : Ω)
-  (p : impure ix α) (f : α -> impure ix β)
-  (respect : respectful_impure c ω p)
-  (run : forall (x : α) (ω' : Ω),
-      respectful_run c p ω ω' x -> respectful_impure c ω' (f x))
-  : respectful_impure c ω (impure_bind p f).
-
-Proof.
-  revert ω respect run.
-  induction p; intros ω respect run.
-  + apply run.
-    constructor.
-  + cbn.
-    inversion respect; ssubst.
-    constructor.
-    ++ apply req.
-    ++ intros y o_callee_x.
-       apply H0; [ auto | ].
-       intros z ω' run'.
-       apply run.
-       econstructor; eauto.
-Qed.
-
-Hint Resolve respectful_bind_respectful_run : freespec.
-
-Lemma respectful_bind_exists_respectful_run `{MayProvide ix i} {α β Ω}
-    (c : contract i Ω) (ω ω' : Ω)
-    (p : impure ix α) (f : α -> impure ix β) (x : β)
-    (respect : respectful_run c (impure_bind p f) ω ω' x)
-  : exists (ω'' : Ω) (y : α),
-    respectful_run c p ω ω'' y /\ respectful_run c (f y) ω'' ω' x.
-
-Proof.
-  revert respect.
-  revert ω ω'.
-  induction p; intros ω ω' respect.
-  + exists ω; exists x0.
-    split.
-    ++ constructor.
-    ++ exact respect.
-  + inversion respect; ssubst.
-    apply H0 in rec.
-    destruct rec as [ω'' [y [trust1 trust2]]].
-    exists ω''; exists y.
-    split; auto.
-    constructor 2 with (x := x0); auto.
-Qed.
-
-#[program]
-Instance respectful_run_Proper
-  : Proper (equal ==> eq ==> eq ==> eq ==> Basics.impl) (@respectful_run ix i H α Ω c).
-
-Next Obligation.
-  add_morphism_tactic.
-  unfold Basics.impl.
-  intros p q equ.
-  induction equ.
-  + intros ω ω' y run.
-    now inversion run; subst.
-  + intros ω ω' y run.
-    inversion run; ssubst.
-    constructor 2 with (x := x).
-    ++ auto.
-    ++ auto.
-    ++ now apply H0.
-Qed.
-
-(** ** Semantics Compliance *)
-
-(** Given a semantics [sem], and a witness [ω] if [sem] computes results which
-    satisfies [c] callee obligations for effects which satisfy [c] caller
-    obligations and if the resulting semantics produces after interpreting [e]
-    complies to [c] in accordance to [ω'], where [ω'] is the new witness state
-    after [e] interpretation then [sem] complies to [c] in accordance to [ω] *)
-
-CoInductive compliant_semantics `{MayProvide ix i} {Ω} (c : contract i Ω) : Ω -> semantics ix -> Prop :=
-| compliant_semantics_rec
-    (sem : semantics ix) (ω : Ω)
-    (o_callee : forall {α} (e : ix α),
-        gen_caller_obligation c ω e -> gen_callee_obligation c ω e (eval_effect sem e))
-    (next : forall {α} (e : ix α),
-        gen_caller_obligation c ω e
-        -> compliant_semantics c (gen_witness_update c ω e (eval_effect sem e)) (exec_effect sem e))
-  : compliant_semantics c ω sem.
-
-(** Proving that semantics obtained from the [store] function are compliant with
-    [store_specs] is relatively simple. *)
-
-Lemma store_complies_to_store_specs {s} (st : s)
-  : compliant_semantics (store_specs s) st (store st).
-
-Proof.
-  revert st; cofix compliant_semantics_rec; intros st.
-  constructor.
-  + intros a [ | st' ] _.
-    ++ now constructor.
-    ++ now constructor.
-  + intros a e req.
-    cbn.
-    assert (R : exec_effect (store st) e = store (store_update s st a e (eval_effect (store st) e)))
-      by now destruct e as [ | st' ].
-    rewrite R.
-    apply compliant_semantics_rec.
-Qed.
-
-Lemma compliant_semantics_caller_obligation_callee_obligation `{MayProvide ix i} {Ω α} (c : contract i Ω) (ω : Ω)
-  (e : ix α) (o_caller : gen_caller_obligation c ω e)
-  (sem : semantics ix) (comp : compliant_semantics c ω sem)
-  : gen_callee_obligation c ω e (eval_effect sem e).
-
-Proof.
-  inversion comp; ssubst.
-  now apply o_callee.
-Qed.
-
-Hint Resolve compliant_semantics_caller_obligation_callee_obligation : freespec.
-
-Lemma compliant_semantics_caller_obligation_compliant `{MayProvide ix i} {Ω α} (c : contract i Ω) (ω : Ω)
-  (e : ix α) (o_caller : gen_caller_obligation c ω e)
-  (sem : semantics ix) (comp : compliant_semantics c ω sem)
-  : compliant_semantics c (gen_witness_update c ω e (eval_effect sem e)) (exec_effect sem e).
-
-Proof.
-  inversion comp; ssubst.
-  now apply next.
-Qed.
-
-Hint Resolve compliant_semantics_caller_obligation_compliant : freespec.
-
-Lemma compliant_semantics_exec_effect_equ `{MayProvide ix i} {Ω α} (c : contract i Ω) (ω : Ω)
-  (sem sem' : semantics ix) (equ : sem === sem')
-  (e : ix α)
-  : exec_effect sem e === exec_effect sem' e.
-
-Proof.
-  inversion equ; ssubst.
-  specialize step_equiv with α e.
-  now inversion step_equiv; ssubst.
-Qed.
-
-Hint Resolve compliant_semantics_exec_effect_equ : freespec.
-
-#[program]
-Instance compliant_semantics_Proper : Proper (equal ==> Basics.impl) (@compliant_semantics ix i H Ω c ω).
-
-Next Obligation.
-  add_morphism_tactic.
-  revert ω.
-  cofix compliant_semantics_Proper; intros ω.
-  intros σ σ' equ comp.
-  destruct comp.
-  constructor.
-  + now setoid_rewrite <- equ.
-  + intros a e o_caller.
-    apply (compliant_semantics_Proper (gen_witness_update c ω e (eval_effect σ' e)) (exec_effect sem e)).
-    ++ auto with freespec.
-    ++ rewrite <- equ at 1.
-       now apply next.
-Qed.
-
-Lemma no_contract_compliant_semantics `{MayProvide ix i} (sem : semantics ix) (u : unit)
-  : compliant_semantics (no_contract i) u sem.
-
-Proof.
-  revert sem.
-  cofix no_contract_compliant_semantics; intros sem.
-  constructor.
-  + trivial.
-  + intros α e req.
-    unfold gen_witness_update.
-    destruct (proj_p e); [ apply no_contract_compliant_semantics | auto ].
-Qed.
-
-Hint Resolve no_contract_compliant_semantics : freespec.
-
-#[local]
-Fixpoint witness_impure_aux `{MayProvide ix i} {Ω α}
-  (sem : semantics ix) (p : impure ix α) (c : contract i Ω) (ω : Ω) : interp_out ix α * Ω :=
-  match p with
-  | local x => (mk_out x sem, ω)
-  | request_then e f =>
-    let out := run_effect sem e in
-    let res := interp_result out in
-    witness_impure_aux (interp_next out) (f res) c (gen_witness_update c ω e res)
-  end.
-
-#[program]
-Instance witness_impure_aux_Proper_2
-  : Proper (eq ==> equal ==> eq ==> eq ==> eq) (@witness_impure_aux ix i H Ω a).
-
-Next Obligation.
-  add_morphism_tactic.
-  intros sem p q equp c ω.
-  revert sem ω.
-  induction equp; intros sem ω.
-  + reflexivity.
-  + cbn.
-    apply H0.
-Qed.
-
-Lemma fst_witness_impure_aux_run_impure `{MayProvide ix i} {Ω α}
-  (sem : semantics ix) (p : impure ix α) (c : contract i Ω) (ω : Ω)
-  : fst (witness_impure_aux sem p c ω) = run_impure sem p.
-
-Proof.
-  revert sem ω.
-  induction p; intros sem ω.
-  + reflexivity.
-  + apply H0.
-Qed.
-
-Hint Rewrite @fst_witness_impure_aux_run_impure : freespec.
-
-Definition witness_impure `{MayProvide ix i} {Ω α}
-  (sem : semantics ix) (p : impure ix α) (c : contract i Ω) (ω : Ω) : Ω :=
-  snd (witness_impure_aux sem p c ω).
-
-#[program]
-Instance witness_impure_Proper
-  : Proper (eq ==> equal ==> eq ==> eq ==> eq) (@witness_impure ix i H Ω α).
-
-Next Obligation.
-  add_morphism_tactic.
-  unfold witness_impure.
-  intros sem p q equp c ω.
-  now rewrite equp.
-Qed.
-
-Lemma compliant_semantics_respectful_impure_gives_respectful_run `{MayProvide ix i} {Ω α}
-  (c : contract i Ω) (ω : Ω) (p : impure ix α) (trust : respectful_impure c ω p)
-  (sem : semantics ix) (comp : compliant_semantics c ω sem)
-  : respectful_run c p ω (witness_impure sem p c ω) (eval_impure sem p).
-
-Proof.
-  revert sem comp trust. revert ω.
-  induction p; intros ω sem comp trust.
-  + constructor.
-  + inversion trust; ssubst.
-    inversion comp; ssubst.
-    econstructor; auto.
-    apply H0.
-    ++ now apply next0.
-    ++ inversion trust; ssubst.
-       apply next1.
-       now apply o_callee.
-Qed.
-
-Hint Resolve compliant_semantics_respectful_impure_gives_respectful_run : freespec.
-
-Lemma witness_impure_request_then_equ `{MayProvide ix i} {Ω α β} (c : contract i Ω) (ω : Ω)
-  (sem : semantics ix) (e : ix α) (f : α -> impure ix β)
-  : witness_impure sem (request_then e f) c ω
-    = witness_impure (exec_effect sem e)
-                     (f (eval_effect sem e))
-                     c
-                     (gen_witness_update c ω e (eval_effect sem e)).
-
-Proof eq_refl.
-
-Hint Rewrite @witness_impure_request_then_equ : freespec.
-
-Lemma respectful_impure_compliant_specs `{MayProvide ix i} {Ω α} (c : contract i Ω) (ω : Ω)
-  (p : impure ix α) (trust : respectful_impure c ω p)
-  (sem : semantics ix) (comp : compliant_semantics c ω sem)
-  : compliant_semantics c (witness_impure sem p c ω) (exec_impure sem p).
-
-Proof.
-  revert trust sem comp. revert ω.
-  induction p; intros ω trust sem comp.
-  + exact comp.
-  + inversion trust; ssubst.
-    autorewrite with freespec.
-    apply H0; auto with freespec.
-Qed.
-
-Hint Resolve respectful_impure_compliant_specs : freespec.
-
-Lemma gen_callee_obligation_equ {α Ωi Ωj} `{Provide ix i} `{Provide ix j}
-    (ci : contract i Ωi) (ωi : Ωi)
-    (cj : contract j Ωj) (ωj : Ωj)
-    (e : ix α) (x : α)
-  : gen_callee_obligation ci ωi e x /\ gen_callee_obligation cj ωj e x
-    <-> gen_callee_obligation (ci + cj) (ωi, ωj) e x.
-
-Proof.
-  split; auto.
-Qed.
-
-Lemma gen_caller_obligation_equ {α Ωi Ωj} `{Provide ix i} `{Provide ix j}
-    (ci : contract i Ωi) (ωi : Ωi) (cj : contract j Ωj) (ωj : Ωj) (e : ix α)
-  : gen_caller_obligation ci ωi e /\ gen_caller_obligation cj ωj e
-    <-> gen_caller_obligation (ci + cj) (ωi, ωj) e.
-
-Proof.
-  split; auto.
-Qed.
-
-Lemma respectful_impure_generalize `{Provide ix i} `{Provide ix j} {α Ωi Ωj}
-    (p : impure ix α)
-    (ci : contract i Ωi) (ωi : Ωi) (cj : contract j Ωj) (ωj : Ωj)
-  : respectful_impure ci ωi p
-    -> respectful_impure cj ωj p
-    -> respectful_impure (ci + cj) (ωi, ωj) p.
-
-Proof.
-  revert ωi ωj.
-  induction p; intros ωi ωj.
-  + intros.
-    constructor.
-  + intros trust trust'.
-    inversion trust; ssubst.
-    inversion trust'; ssubst.
-    constructor.
-    ++ rewrite <- gen_caller_obligation_equ.
-       now split.
-    ++ intros x o_callee.
-       rewrite <- gen_callee_obligation_equ in o_callee.
-       apply H3; [ apply next | apply next0 ]; apply o_callee.
-Qed.
-
-(** ** Component Correctness *)
-
-(** We consider a component [c : component i j s], meaning [c] exposes an
-    interface [i], uses an interface [j], and carries an internal state of type
-    [s].
-
-<<
-                            c : component i j s
-                        i +---------------------+      j
-                        | |                     |      |
-                +------>| |       st : s        |----->|
-                        | |                     |      |
-                          +---------------------+
->>
-
-    We say [c] is correct wrt. [ci] (a contract for [i]) and [cj] (a contract
-    for [i]) iff given primitives which satisfies the caller obligation of [ci],
-    [c] will
-
-    - use respectful impure computations wrt. [cj]
-    - compute results which satisfy [ci] callee obligations, assuming it can
-      rely on a semantics of [j] which complies with [cj]
-
-    The two witness states [ωi : Ωi] (for [speci]) and [ωj : Ωj] (for [specj]),
-    and [st : s] the internal state of [c] remained implicit in the previous
-    sentence.  In practice, we associate them together by means of a dedicated
-    predicate [pred].  It is expected that [pred] is an invariant throughout
-    [c]'s life, meaning that as long as [c] computes result for legitimate
-    effects (wrt.  [speci] effects, the updated values of [ωi], [ωj] and [st]
-    continue to satisfy [pred]. *)
-
-Definition correct_component {i jx Ωi Ωj}
-  (c : component i jx) `{MayProvide jx j}
-  (ci : contract i Ωi) (cj : contract j Ωj)
-  (pred : Ωi -> Ωj -> Prop) : Prop :=
-  forall (ωi : Ωi) (ωj : Ωj) (init : pred ωi ωj)
-    (α : Type) (e : i α) (o_caller : caller_obligation ci ωi e),
-    respectful_impure cj ωj (c α e) /\
-    forall (x : α) (ωj' : Ωj)
-      (run : respectful_run cj (c α e) ωj ωj' x),
-      callee_obligation ci ωi e x /\ pred (witness_update ci ωi e x) ωj'.
-
-(** Once we have proven [c] is correct wrt. to [speci] and [specj] with [pred]
-    acting as an invariant throughout [c] life, we show we can derive a
-    semantics from [c] with an initial state [st] which complies to [speci] in
-    accordance to [ωi] if we use a semantics of [j] which complies to [specj] in
-    accordance to [ωj], where [pred ωi st ωj] is satisfied. *)
-
-Lemma respectful_impure_compliant_specs_respectful_run `{MayProvide ix i} {a Ω}
-    (spec : contract i Ω) (ω : Ω)
-    (sem : semantics ix) (comp : compliant_semantics spec ω sem)
-    (p : impure ix a) (trust : respectful_impure spec ω p)
-  : respectful_run spec p ω (witness_impure sem p spec ω) (eval_impure sem p).
-
-Proof.
-  revert ω sem comp trust.
-  induction p; intros ω sem comp trust.
-  + constructor.
-  +  inversion trust; ssubst.
-     constructor 2 with (x := eval_effect sem e).
-     ++ exact req.
-     ++ auto with freespec.
-     ++ change (witness_impure sem (request_then e f) spec ω)
-          with (witness_impure (exec_effect sem e) (f (eval_effect sem e)) spec
-                               (gen_witness_update spec ω e (eval_effect sem e))).
-        change (eval_impure sem (request_then e f))
-          with (eval_impure (exec_effect sem e) (f (eval_effect sem e))).
-        apply H0;
-          auto with freespec.
-Qed.
-
-Lemma correct_component_derives_compliant_semantics `{MayProvide jx j} {i Ωi Ωj}
-  (c : component i jx) (ci : contract i Ωi) (cj : contract j Ωj)
-  (pred : Ωi -> Ωj -> Prop)
-  (correct : correct_component c ci cj pred)
-  (ωi : Ωi) (ωj : Ωj) (inv : pred ωi ωj)
-  (sem : semantics jx) (comp : compliant_semantics cj ωj sem)
-  : compliant_semantics ci ωi (derive_semantics c sem).
-
-Proof.
-  revert ωi ωj inv sem comp.
-  cofix correct_component_derives_compliant_semantics.
-  intros ωi ωj inv sem comp.
-  unfold correct_component in correct.
-  specialize (correct ωi ωj inv).
-  constructor; intros a e req; specialize (correct a e req);
-    destruct correct as [trust run].
-    specialize run with (eval_impure sem (c a e))
-                        (witness_impure (H := H) sem (c a e) cj ωj).
-  + apply run.
-    auto with freespec.
-  + eapply correct_component_derives_compliant_semantics.
-    ++ apply run.
-       apply respectful_impure_compliant_specs_respectful_run; auto.
-    ++ fold (exec_impure sem (c a e)).
-       auto with freespec.
-Qed.
