theories/Core/Hoare.v
@@ -18,123 +18,64 @@
  * along with this program. If not, see <http://www.gnu.org/licenses/>.
  *)
 
-From Base Require Export Prelude.
-From FreeSpec Require Import Impure Contract Morphism Tactics.
+From ExtLib Require Import Functor Applicative Monad.
+From FreeSpec.Core Require Import Interface Impure Contract.
 
-(** If we consider the monad form by the set of sets of predicates, that is
+(** * Definition *)
 
-<<
-Definition predicate (a : Type) : Type := a -> Prop.
->>
+Record hoare (Σ : Type) (α : Type) : Type :=
+  mk_hoare { pre : Σ -> Prop
+           ; post : Σ -> α -> Σ -> Prop
+           }.
 
-    whose [bind] and [pure] functions is defined as follows
+Arguments mk_hoare {Σ α} (pre post).
+Arguments pre {Σ α} (_ _).
+Arguments post {Σ α} (_ _ _).
 
-<<
-Definition predicat_bind {α β} (p : predicate α) (f : α -> predicate β)
-  : predicate β :=
-  fun r => exists (x : α), p x /\ (f x) r.
+Definition hoare_pure {Σ α} (x : α) : hoare Σ α :=
+  mk_hoare (fun _ => True) (fun s y s' => x = y /\ s = s').
 
-Definition predicat_pure {α} (x : α) : predicate α := eq x.
->>
+Definition hoare_bind {Σ α β} (h : hoare Σ α) (k : α -> hoare Σ β) : hoare Σ β :=
+  mk_hoare (fun s => pre h s /\ (forall x s', post h s x s' -> pre (k x) s'))
+           (fun s x s'' => exists y s', post h s y s' /\ post (k y) s' x s'').
 
-    Then, given [f := fun α e => fun x => True] the morphism from the interface
-    type [i] to [predicate] such that [f α e] is a predicate which is always
-    satisfied, [morphism_lift f p] is a predicate which allows for reasoning
-    about any potential output of [p] (that is, considering any implementer for
-    [i]).
+(** * Instances *)
 
-    The [hoare] monad is another interesting candidate for reifying our [impure]
-    monad, and we demonstrate here that we can easily provide a morphism from
-    [impure] to [hoare], to the extent that we provide a contract to generate
-    the [pre] and [post] condition of the hoare monad.
+(** ** Functor *)
 
-    We define the [hoare_of_contract] morphism parameterized by a contract [c]
-    to project primitives of an interface to the [hoare] monad. This morphism
-    use the obligations of [c] to define the precondition and postcondition of
-    the resulting [hoare] monadic term. *)
+Definition hoare_map {Σ α β} (f : α -> β) (h : hoare Σ α) : hoare Σ β :=
+  hoare_bind h (fun x => hoare_pure (f x)).
 
-Definition hoare_of_contract `{MayProvide ix i} {Ω} (c : contract i Ω)
-  : ix ~> hoare Ω :=
-  fun α (e : ix α) =>
-    mk_hoare (fun ω => gen_caller_obligation c ω e)
-             (fun ω x ω' =>
-                gen_callee_obligation c ω e x
-                /\ ω' = gen_witness_update c ω e x).
+Instance hoare_Functor Σ : Functor (hoare Σ) :=
+  { fmap := fun _ _ => hoare_map }.
 
-Definition hoare_of_impure `{MayProvide ix i} {Ω} (c : contract i Ω)
+(** ** Applicative *)
+
+Definition hoare_apply {Σ α β} (hf : hoare Σ (α -> β)) (h : hoare Σ α)
+  : hoare Σ β :=
+  hoare_bind hf (fun f => hoare_map f h).
+
+Instance hoare_Applicative : Applicative (hoare Σ) :=
+  { ap := fun _ _ => hoare_apply
+  ; pure := fun _ => hoare_pure
+  }.
+
+(** ** Monad *)
+
+Instance hoare_Monad Σ : Monad (hoare Σ) :=
+  { ret := @hoare_pure Σ; bind := @hoare_bind Σ }.
+
+(** * Lift *)
+
+Definition interface_to_hoare `{MayProvide ix i} `(c : contract i Ω) : ix ~> hoare Ω :=
+  fun a e =>
+    {| pre := fun ω => gen_caller_obligation c ω e
+     ; post := fun ω x ω' => gen_callee_obligation c ω e x
+                             /\ ω' = gen_witness_update c ω e x
+    |}.
+
+Definition to_hoare `{MayProvide ix i} `(c : contract i Ω)
   : impure ix ~> hoare Ω :=
-  morphism_lift (hoare_of_contract c).
+  impure_lift (interface_to_hoare c).
 
-Arguments hoare_of_impure {ix i H Ω} (c) {α} _.
-
-(** Then, we demonstrate that, considering [hp] the (hoare) monad computed
-    thanks to [hoare_of_contract] and [morphism_lift], and an impure computation
-    [p]
-
-      - [respectful_impure_equivalence]: If a witness state [ω] satisfies the
-        pre condition of [hp], then [p] is respectful wrt. [c] in accordance to
-        [ω] (see [respectful_impure]).
-      - [respectful_run_equivalence]: Similarly, if a tuple [(ω, x, ω')]
-        satisfies the post condition [hp], then there exists a respectful run
-        from [ω] to compute [x] and [ω'] (see [respectful_run]). *)
-
-Lemma respectful_impure_equivalence  `{MayProvide ix i} {α Ω}
-    (c : contract i Ω) (ω : Ω) (p : impure ix α)
-  : respectful_impure c ω p <-> pre (hoare_of_impure c p) ω.
-
-Proof.
-  revert ω.
-  induction p; intros ω.
-  + split; cbn.
-    ++ auto.
-    ++ intros _.
-       constructor.
-  + cbn.
-    split.
-    ++ intros r.
-       inversion r; ssubst.
-       split; [ exact req | ].
-       intros x s'.
-       intros [post equ].
-       specialize next with x.
-       apply next in post.
-       apply H0 in post.
-       rewrite equ.
-       apply post.
-    ++ intros [p r1].
-       constructor; [ exact p | ].
-       intros x q.
-       rewrite H0.
-       apply r1.
-       split; [ exact q | reflexivity ].
-Qed.
-
-Lemma respectful_run_equivalence  `{MayProvide ix i} {α Ω}
-    (c : contract i Ω) (p : impure ix α) (ω : Ω) (x : α) (ω' : Ω)
-    (h : respectful_impure c ω p)
-  : respectful_run c p ω ω' x <-> post (hoare_of_impure c p) ω x ω'.
-
-Proof.
-  revert ω ω' x h.
-  induction p; intros ω ω' r h.
-  + split; cbn.
-    ++ intros run.
-       unroll_respectful_run run; auto.
-    ++ intros [r1 r2].
-       subst.
-       constructor.
-  + inversion h; ssubst.
-    split.
-    ++ intros run.
-       inversion run; ssubst.
-       cbn.
-       exists x.
-       exists (gen_witness_update c ω e x).
-       repeat split; auto.
-       apply H0; auto.
-    ++ intros [t [ω'' [[r1 r2] r3]]]; subst.
-       econstructor.
-       +++ apply req.
-       +++ apply r1.
-       +++ apply H0; auto.
-Qed.
+Arguments to_hoare {ix i _ Ω} c {α} _.
