theories/Core/Core.v
@@ -1,8 +1,8 @@
 (* FreeSpec
- * Copyright (C) 2018–2019 ANSSI
+ * Copyright (C) 2018–2020 ANSSI
  *
  * Contributors:
- * 2018–2019 Thomas Letan <thomas.letan@ssi.gouv.fr>
+ * 2018–2020 Thomas Letan <thomas.letan@ssi.gouv.fr>
  *
  * This program is free software: you can redistribute it and/or modify
  * it under the terms of the GNU General Public License as published by
@@ -18,5 +18,11 @@
  * along with this program. If not, see <http://www.gnu.org/licenses/>.
  *)
 
-From Base Require Export Prelude.
-From FreeSpec.Core Require Export Interface Impure Semantics Contract Tactics.
+From FreeSpec.Core Require Export
+     Interface
+     Impure
+     Semantics
+     Component.
+
+#[global]
+Open Scope freespec_scope.
