theories/Core/Extraction.v
@@ -1,13 +1,3 @@
-From FreeSpec.Core Require Import All.
+From FreeSpec Require Import Core.
 
 Extraction Inline impure_Applicative.
-
-Class HasMLImpl ix :=
-  { ml_semantics : semantics ix }.
-
-Instance ExtractiblePlus `(HasMLImpl i, HasMLImpl j)
-  : HasMLImpl (i + j) :=
-  { ml_semantics := ml_semantics * ml_semantics }.
-
-Definition gen_main {α} `{HasMLImpl ix} : impure ix α -> α :=
-  eval_impure ml_semantics.
