theories/Core/Hoare/hoare_tactics.v
@@ -1,0 +1,132 @@
+(** Reasoning with the [hoare] type has proven to be cumbersome to say the
+    least. However, one can use the automation features of Coq to ease the
+    verification process.
+
+    More precisely, we implement several “angry”, ad-hoc tactics. *)
+
+Lemma iff_p_p (p : Prop) : (p <-> p) <-> True.
+
+Proof.
+  now split.
+Qed.
+
+Lemma prop_and_neutral (p : Prop) : (True /\ p) <-> p.
+
+Proof.
+  now repeat split.
+Qed.
+
+Lemma imply_true_true (p : Type) : (p -> True) <-> True.
+
+Proof.
+  now repeat split.
+Qed.
+
+Lemma and_imply_equ (p q r : Prop) : (p /\ q -> r) <-> (p -> q -> r).
+
+Proof.
+  split.
+  + intros H hp hq.
+    apply H.
+    now split.
+  + intros H [hp hq].
+    now apply H.
+Qed.
+
+Lemma alias_equ {a} (x : a) (p : a -> Prop)
+  : (forall (y : a), y = x -> p y) <-> p x.
+
+Proof.
+  split.
+  + intros H.
+    now apply (H x).
+  + intros hx y equ.
+    now rewrite equ.
+Qed.
+
+Lemma forall_equ_2 {a b} (x : a) (y : b) (p : a -> b -> Prop)
+  : (forall (x' : a) (y' : b), x = x' -> y = y' -> p x' y') <-> p x y.
+
+Proof.
+  split.
+  + intros H.
+    now apply H.
+  + intros hxy x' y' equ1 equ2.
+    now subst.
+Qed.
+
+Lemma forall_equ_2' {a b} (x : a) (y : b) (p : a -> b -> Prop)
+  : (forall (x' : a) (y' : b), x' = x -> y' = y -> p x' y') <-> p x y.
+
+Proof.
+  split.
+  + intros H.
+    now apply H.
+  + intros hxy x' y' equ1 equ2.
+    now subst.
+Qed.
+
+Lemma exists_equ_2 {a b} (x : a) (y : b) (p : a -> b -> Prop)
+  : (exists (x' : a) (y' : b), (x = x' /\ y = y') /\ p x' y') <-> p x y.
+
+Proof.
+  split.
+  + intros H.
+    now destruct H as [x' [y' [[equ1 equ2] H]]]; subst.
+  + intros hxy.
+    exists x.
+    exists y.
+    now split.
+Qed.
+
+Lemma exists_equ_2' {a b} (x : a) (y : b) (p : a -> b -> Prop)
+  : (exists (x' : a) (y' : b), (x' = x /\ y' = y) /\ p x' y') <-> p x y.
+
+Proof.
+  split.
+  + intros H.
+    now destruct H as [x' [y' [[equ1 equ2] H]]]; subst.
+  + intros hxy.
+    exists x.
+    exists y.
+    now split.
+Qed.
+
+Lemma eq_sym_equ {a} (x y : a) : x = y <-> y = x.
+
+Proof.
+  now repeat split.
+Qed.
+
+Ltac angry_rewrite :=
+  repeat (
+      setoid_rewrite prop_and_neutral
+      || setoid_rewrite imply_true_true
+      || setoid_rewrite (and_comm _ True)
+      || setoid_rewrite (and_comm _ (_ /\ _))
+      || setoid_rewrite and_imply_equ
+      || setoid_rewrite forall_equ_2
+      || setoid_rewrite exists_equ_2
+      || setoid_rewrite exists_equ_2'
+      || setoid_rewrite iff_p_p
+    ).
+
+Ltac angry_destruct H :=
+  match type of H with
+  | _ /\ _ => let H' := fresh "H" in
+              let H'' := fresh "H" in
+              destruct H as [H' H''];
+              angry_destruct H';
+              angry_destruct H''
+  | exists _, _ => let x := fresh "x" in
+                   let H' := fresh "H" in
+                   destruct H as [x H']; angry_destruct H'
+  | _ => idtac
+  end.
+
+Ltac angry_intros :=
+  let H := fresh "H" in
+  intros H; angry_destruct H.
+
+Ltac angry_exists :=
+  repeat (eexists; eauto).
