theories/Core/ImpureFacts.v
@@ -1,0 +1,163 @@
+From FreeSpec.Core Require Export Impure.
+
+(** ** Equivalence *)
+
+(** Due to the definition of [impure] and [impure_bind], we could decide to rely
+    on Coq built-in [eq] to reason about impure computations equivalence, but we
+    would have to use the functional extensionality axiom to handle the
+    continuation of the [request_then] constructor. In order to keep FreeSpec
+    axiom-free, we rather provide a custom equivalence for [impure] terms.
+
+    The definition of [impure_equiv] is two-fold. *)
+
+Inductive impure_eq {i α} : impure i α -> impure i α -> Prop  :=
+
+(** - Two impure computations are equivalent if and only if they compute the
+      exact same term (wrt. Coq [eq] function). *)
+
+| local_eq (x : α) : impure_eq (local x) (local x)
+
+(** - Two computations which consist in requesting the interpretation of an
+      primitive and passing the result to a monadic continuation are equivalent
+      if and only if they use the exact same primitive in the first place, and
+      given any result the interpretation of this primitive may produce, their
+      continuation returns equivalent impure computations. *)
+
+| request_eq {β} (e : i β) (f g : β -> impure i α)
+    (equ : function_eq impure_eq f g)
+  : impure_eq (request_then e f) (request_then e g).
+
+Infix "===" := impure_eq : impure_scope.
+
+(** The definition of [impure_equiv] is very similar to [eq], with the exception
+    of the treatment of the continuation. There is no much effort to put into
+    proving this is indeed a proper equivalence. *)
+
+#[program]
+Instance impure_Equivalence : @Equivalence (impure i α) impure_eq := {}.
+
+Next Obligation.
+  intros p.
+  induction p; constructor.
+  intros x.
+  apply H.
+Qed.
+
+Next Obligation.
+  intros p q equ.
+  induction equ; constructor.
+  intros x.
+  apply H.
+Qed.
+
+Next Obligation.
+  intros p q r pq qr.
+  revert p r pq qr.
+  induction q; intros p r pq qr.
+  + inversion pq; ssubst; inversion qr; ssubst.
+    constructor.
+  + inversion pq; ssubst; inversion qr; ssubst.
+    constructor.
+    intros x.
+    cbv in H.
+    now apply H with (β := x).
+Qed.
+
+#[program]
+Instance request_then_Proper
+  : Proper (eq ==> function_eq impure_eq ==> impure_eq) (@request_then i α β).
+
+Next Obligation.
+  add_morphism_tactic.
+  intros e f g equ.
+  constructor.
+  intros y.
+  specialize (equ y).
+  now rewrite equ.
+Qed.
+
+#[program]
+Instance impure_bind_Proper
+  : Proper (impure_eq ==> function_eq impure_eq ==> impure_eq) (@impure_bind i α β).
+
+Next Obligation.
+  add_morphism_tactic.
+  intros x y equ1 f g equ2.
+  induction equ1.
+  + cbn.
+    now rewrite (equ2 x).
+  + cbn.
+    constructor.
+    intros x.
+    apply H.
+Qed.
+
+Ltac change_request_then :=
+  match goal with
+  | |- (request_then ?e ?f === request_then ?e ?g)%impure =>
+    let R := fresh "R" in
+    assert (R: function_eq impure_eq f g); [ intros ?x | rewrite R; clear R ]
+  end.
+
+Ltac change_impure_bind :=
+  match goal with
+  | |- (impure_bind ?e ?f === impure_bind ?e ?g)%impure =>
+    let R := fresh "R" in
+    assert (R: function_eq impure_eq f g); [ intros ?x | now rewrite R ]
+  end.
+
+Lemma impure_bind_local {i α} (p : impure i α)
+  : (impure_bind p (fun x => local x) === p)%impure.
+
+Proof.
+  induction p.
+  + reflexivity.
+  + cbn.
+    change_request_then; [ | reflexivity ].
+    now rewrite H.
+Qed.
+
+Lemma impure_bind_assoc {i α β δ}
+  (p : impure i α) (f : α -> impure i β) (g : β -> impure i δ)
+  : (impure_bind (impure_bind p f) g
+     === impure_bind p (fun x => impure_bind (f x) g))%impure.
+
+Proof.
+  induction p; [reflexivity | ].
+  cbn.
+  change_request_then; auto.
+  reflexivity.
+Qed.
+
+Instance impure_map_Proper
+  : Proper (function_eq eq ==> impure_eq ==> impure_eq) (@impure_map i α β).
+
+Proof.
+  add_morphism_tactic.
+  intros f g equf p q equp.
+  unfold impure_map.
+  rewrite equp.
+  change_impure_bind.
+  now rewrite equf.
+Qed.
+
+#[program]
+Instance impure_apply_Proper
+  : Proper (impure_eq ==> impure_eq ==> impure_eq) (@impure_apply i α β).
+
+Next Obligation.
+  add_morphism_tactic.
+  intros p q equ1 r s equ2.
+  unfold impure_apply.
+  rewrite equ1.
+  change_impure_bind.
+  cbn.
+  now rewrite equ2.
+Qed.
+
+Lemma bind_request_then_assoc `(e : i a) `(f : a -> impure i b) `(g : b -> impure i c)
+  : request_then e f >>= g = request_then e (fun x => f x >>= g).
+
+Proof.
+  reflexivity.
+Qed.
