theories/Core/Init.v
@@ -1,0 +1,80 @@
+(** * Coq Set-up *)
+
+#[global] Generalizable All Variables.
+
+(** * Coq Stdlib Notations *)
+
+From Coq Require Export List RelationClasses Setoid Morphisms.
+Export ListNotations.
+
+#[global] Open Scope signature_scope.
+#[global] Close Scope nat_scope.
+#[global] Open Scope bool_scope.
+
+
+(** * ExtLib Notations *)
+
+From ExtLib Require Export Functor Applicative Monad.
+Export FunctorNotation.
+Export ApplicativeNotation.
+Export MonadLetNotation.
+
+#[global] Open Scope monad_scope.
+
+From ExtLib Require Export Extras.
+Export FunNotation.
+
+Definition when {m : Type -> Type} `{Monad m} (cond : bool) `(p : m a) : m unit :=
+  if cond then (p;; pure tt) else pure tt.
+
+(** * Tactics *)
+
+From Coq Require Export Eqdep.
+
+Ltac ssubst :=
+  lazymatch goal with
+| [ H : existT _ _ _ = existT _ _ _ |- _ ]
+  => apply Eqdep.EqdepTheory.inj_pair2 in H; ssubst
+| [ |- _] => subst
+end.
+
+(** * Notations *)
+
+Declare Scope freespec_scope.
+Delimit Scope freespec_scope with freespec.
+
+Reserved Infix "===" (at level 70, no associativity).
+
+Notation "m '~>' n" :=
+  (forall (α : Type), m α -> n α)
+    (at level 80, no associativity)
+  : type_scope.
+
+(** * Generalizable Functions Equality *)
+
+Definition function_eq {a b} (r : b -> b -> Prop) (f g : a -> b) : Prop :=
+  forall (x : a), r (f x) (g x).
+
+#[program]
+Instance function_eq_Equivalence `(Equivalence b r)
+  : @Equivalence (a -> b) (function_eq r).
+
+Next Obligation.
+  now intros f x.
+Qed.
+
+Next Obligation.
+  intros f g equ x.
+  symmetry.
+  apply equ.
+Qed.
+
+Next Obligation.
+  intros f g h equ1 equ2 x.
+  transitivity (g x); [ apply equ1 | apply equ2 ].
+Qed.
+
+(** * Hint Databases *)
+
+#[global]
+Create HintDb freespec.
