theories/Core/Instrument.v
@@ -1,0 +1,23 @@
+From ExtLib Require Import StateMonad MonadTrans.
+From FreeSpec.Core Require Import Interface Semantics Contract.
+
+#[global]
+Notation instrument Ω i := (stateT Ω (state (semantics i))).
+
+Definition interface_to_instrument `{MayProvide ix i} `(c : contract i Ω)
+  : ix ~> instrument Ω ix :=
+  fun a e =>
+    let* x := lift $ interface_to_state _ e in
+    modify (fun ω => gen_witness_update c ω e x);;
+    ret x.
+
+Definition to_instrument `{MayProvide ix i} `(c : contract i Ω)
+  : impure ix ~> instrument Ω ix :=
+  impure_lift $ interface_to_instrument c.
+
+Arguments to_instrument {ix i _ Ω} (c) {α}.
+
+Definition instrument_to_state {i} `(ω : Ω) : instrument Ω i ~> state (semantics i) :=
+  fun a instr => fst <$> runStateT instr ω.
+
+Arguments instrument_to_state {i Ω} (ω) {α}.
