theories/Core/SemanticsFacts.v
@@ -1,0 +1,108 @@
+From ExtLib Require Import StateMonad.
+
+From FreeSpec.Core Require Import Impure Contract.
+From FreeSpec.Core Require Export Semantics.
+
+(** * Semantics Compliance *)
+
+(** Given a semantics [sem], and a witness [ω] if [sem] computes results which
+    satisfies [c] callee obligations for effects which satisfy [c] caller
+    obligations and if the resulting semantics produces after interpreting [e]
+    complies to [c] in accordance to [ω'], where [ω'] is the new witness state
+    after [e] interpretation then [sem] complies to [c] in accordance to [ω] *)
+
+CoInductive compliant_semantics `{MayProvide ix i} `(c : contract i Ω)
+  : Ω -> semantics ix -> Prop :=
+| compliant_semantics_rec
+    (sem : semantics ix) (ω : Ω)
+    (o_callee : forall {α} (e : ix α),
+        gen_caller_obligation c ω e -> gen_callee_obligation c ω e (eval_effect sem e))
+    (next : forall {α} (e : ix α),
+        gen_caller_obligation c ω e
+        -> compliant_semantics c (gen_witness_update c ω e (eval_effect sem e)) (exec_effect sem e))
+  : compliant_semantics c ω sem.
+
+(** Proving that semantics obtained from the [store] function are compliant with
+    [store_specs] is relatively simple. *)
+
+Lemma store_complies_to_store_specs {s} (st : s)
+  : compliant_semantics (store_specs s) st (store st).
+
+Proof.
+  revert st; cofix compliant_semantics_rec; intros st.
+  constructor.
+  + intros a [ | st' ] _.
+    ++ now constructor.
+    ++ now constructor.
+  + intros a e req.
+    cbn.
+    replace (exec_effect (store st) e)
+      with (store (store_update s st a e (eval_effect (store st) e)))
+      by now destruct e as [| st'].
+    apply compliant_semantics_rec.
+Qed.
+
+Hint Resolve store_complies_to_store_specs : freespec.
+
+Lemma compliant_semantics_caller_obligation_callee_obligation `{MayProvide ix i}
+   `(c : contract i Ω) (ω : Ω)
+   `(e : ix α) (o_caller : gen_caller_obligation c ω e)
+    (sem : semantics ix) (comp : compliant_semantics c ω sem)
+  : gen_callee_obligation c ω e (eval_effect sem e).
+
+Proof.
+  inversion comp; ssubst.
+  now apply o_callee.
+Qed.
+
+Hint Resolve compliant_semantics_caller_obligation_callee_obligation : freespec.
+
+Lemma compliant_semantics_caller_obligation_compliant `{MayProvide ix i} {Ω α} (c : contract i Ω) (ω : Ω)
+  (e : ix α) (o_caller : gen_caller_obligation c ω e)
+  (sem : semantics ix) (comp : compliant_semantics c ω sem)
+  : compliant_semantics c (gen_witness_update c ω e (eval_effect sem e)) (exec_effect sem e).
+
+Proof.
+  inversion comp; ssubst.
+  now apply next.
+Qed.
+
+Hint Resolve compliant_semantics_caller_obligation_compliant : freespec.
+
+Lemma no_contract_compliant_semantics `{MayProvide ix i} (sem : semantics ix) (u : unit)
+  : compliant_semantics (no_contract i) u sem.
+
+Proof.
+  revert sem.
+  cofix no_contract_compliant_semantics; intros sem.
+  constructor.
+  + intros α e req.
+    unfold gen_caller_obligation, gen_callee_obligation.
+    destruct proj_p; constructor.
+  + intros α e req.
+    unfold gen_witness_update.
+    destruct (proj_p e); [ apply no_contract_compliant_semantics | auto with freespec ].
+Qed.
+
+Hint Resolve no_contract_compliant_semantics : freespec.
+
+#[program]
+Instance compliant_semantics_Proper `{MayProvide ix i} `(c : contract i Ω)
+  : Proper (eq ==> semantics_eq ==> Basics.impl) (compliant_semantics c).
+
+Next Obligation.
+  add_morphism_tactic.
+  unfold Basics.impl.
+  cofix proper.
+  intros ω sem sem' equ comp.
+  inversion equ; subst.
+  inversion comp; subst.
+  constructor; intros a e pre.
+  + rewrite <- res_eq.
+    now apply o_callee.
+  + specialize next_eqv with a e.
+    eapply proper.
+    exact next_eqv.
+    rewrite <- res_eq.
+    now apply next.
+Qed.
